\documentclass[11pt,oneside,titlepage]{book}
\title{My set theory exercises}
\usepackage{amsmath, amssymb}
\usepackage{geometry}
\usepackage{hyperref}
\author{Evgeny Markin}
\date{2023}

\DeclareMathOperator \map {\mathcal {L}}
\DeclareMathOperator \pow {\mathcal {P}}
\DeclareMathOperator \ns {null}
\DeclareMathOperator \range {range}
\DeclareMathOperator \inv {^{-1}}
\DeclareMathOperator \Span {span}
\DeclareMathOperator \lra {\Leftrightarrow}
\DeclareMathOperator \eqv {\Leftrightarrow}
\DeclareMathOperator \la {\Leftarrow}
\DeclareMathOperator \ra {\Rightarrow}
\DeclareMathOperator \imp {\Rightarrow}
\DeclareMathOperator \true {true}
\DeclareMathOperator \false {false}
\DeclareMathOperator \dom {dom}
\DeclareMathOperator \ran {ran}
\newcommand{\eangle}[1]{\langle #1 \rangle}


\begin{document}
\maketitle
\tableofcontents

\chapter*{Useful things}

I think that it is pretty straightforward to define some function based on axioms that we get.
For example pairing axiom allows us to define $PA: S \times S \to S$ by
$$PA(u, v) = \{u, v\}$$
same goes for union axiom
$$UA(u) = \{\text{elements of elements of U}\}$$
Later some other function might be defined in the same manner.

In logic notation, I denote tautology as '$\true$' and contradiction as '$\false$'

There is a rule that I've used
$$a \land (b \lor \neg a) \lra (a \land b) \lor (a \land \neg a))
\lra (a \land b) \lor (\false) \lra a \land b$$
which I don't remember seeing in the book, but it's pretty useful.

\chapter{Introduction}

\section{Elementary Set Theory}

Let A, B, C be \subsection{}

\textit{If $a \notin A \setminus B$ and $a \in A$, show that $a \in B$}

Because $a \notin A \setminus B$, we follow that $x \in B$ or $x \notin A$. Since $x \in A$, we
follow that $x \in B$, as desired.

\subsection{}

\textit{Show that if $A \subseteq B$, then $C \setminus B \subseteq C \setminus A$}

Let $c \in C \setminus B$. Then we follow that $c \in C$ or $c \notin B$. Since $A \subseteq B$,
we follow that $c \notin B$ implies that $c \notin A$. Thus we follow that
$c \in C \setminus B$ implies that $c \in C \setminus A$. Therefore $C \setminus B \subseteq
C \setminus A$.

\subsection{}

\textit{Suppose $A \setminus B \subseteq C$. Show that $A \setminus C \subseteq B$.}

Suppose that $a \in A \setminus C$. Then we follow that $a \in A$ and $a \notin C$.

Given that $A \setminus B \subseteq C$ and $A \notin C$, we follow that $a \notin A \setminus B$.
Thus $a \notin A$ or $a \in B$. Since $a \in A$, we follow that $a \in B$. Thus
$$a \in A \setminus C \to a \in B$$
$$A \setminus C \subseteq  B$$
as desired.

\subsection{}

\textit{Suppose $A \subseteq B$ and $A \subseteq C$. Show that $A \subseteq B \cap C$}

Suppose that $a \in A$. Then we follow that $a \in B$ and $a \in C$. Thus $a \in B \cap C$.
Therefore we follow that $A \subseteq B \cap C$.

\subsection{}

\textit{Suppose $A \subseteq B$ and $B \cap C = \emptyset$. Show that $A \in B \setminus C$}

Suppose that $a \in A$. Then we follow that $a \in B$ and since $B \cap C = \emptyset$, we
follow that $a \notin C$. Thus $a \in B \setminus C$ by definition. Therefore
$A \subseteq B \setminus C$.

\subsection{}

\textit{Show that $A \setminus (B \setminus C) \subseteq (A \setminus B) \cup C$.}
Suppose that $a \in A \setminus (B \setminus C)$. Then we follow that
$a \in A$ and $a \notin B \setminus C$. Thus $a \notin B$ and $a \in C$. Thus we
follow that $a \in A \setminus B$ or $a \in C$. Thus
$A \setminus (B \setminus C) \subseteq (A \setminus B) \cup C$
as desired.

\subsection{}

\textit{Let $P(x)$ be the property $x > \frac 1 x$. Are the assertions $P(2)$, $P(-2)$,
  $P(\frac 1 2)$ $P( \frac{-1}{2})$ true or false .}

$$2 > \frac 1 2 \to P(2) = true$$
$$-2 < \frac{-1}{2} \to P(-2) = false$$
last two are reversed.

\subsection{}

\textit{Sow that each of the following sets can be expressed as an interval}

$$a) (-3, 3)$$
$$b) (-3, \infty)$$
$$c) (-3, 3)$$

all of them follow from order properties of real numbers.

\subsection{}

\textit{Express the following sets as truth sets}

$$A = \{1, 4, 9, 16, 25, ...\} \iff A = \{x \in N: x = y^2 \textit{ for some } y \in N\}$$
$$B = \{..., -15, -10, -5, 0, 5, ... \} \iff A = \{x \in N: x = 5y  \textit{ for some } y \in N\}$$

\textit{Rest are also trivial, not gonna go deep here}

\section{Logical Notation}

\subsection*{1.2.1}

\textit{Using truth tables, show that $\neg(P \ra Q) \lra (P \land \neg Q)$}

\begin{center}
  \begin{tabular}{c| c| c| c| c| c|}
    P & Q & $P \ra Q$ & $\neg(P \ra Q)$ & $\neg Q$ & $P \land \neg Q$ \\
    false & false & true & false & true & false \\
    false & true & true & false & false & false \\
    true & false & false & true & true & true \\
    true & true & true & false & false & false \\
  \end{tabular}  
\end{center}

from this we can see that they are equqivalent.

\textit{Following 4 exercises are the same as this one, so I'm skipping them}

\subsection*{1.2.5}

\textit{Show that $(P \imp Q) \land (P \imp R) \eqv P \imp (Q \land R)$, using logic laws}

$$(P \imp Q) \land (P \imp R) \eqv (\neg P \lor Q) \land (\neg P \lor R) \eqv
\neg P  \lor (R \land Q) \eqv  P  \imp (R \land Q) $$
Laws used: 
$$CL \to DIST \to CL$$

\subsection*{1.2.6}

\textit{Show that $(P \imp R) \lor (Q \imp R) \eqv (P \land Q) \imp R$, using logic laws}

$$(P \imp R) \lor (Q \imp R)  \eqv (\neg P \lor R) \lor (\neg Q \lor R) \eqv
\neg P \lor R \lor \neg Q \lor R \eqv (\neg Q \lor \neg P) \lor R \eqv$$
$$ \eqv \neg (Q \land P) \lor R
\eqv (Q \land R) \imp R$$
Laws used:
$$CL \to ASC \to ID, ASC \to DML \to CL$$

\subsection*{1.2.7}

\textit{Show that $P \imp (Q \imp R) \eqv (P \land Q) \imp R$, using logic laws}

$$P \imp (Q \imp R) \eqv \neg P \lor (Q \imp R) \eqv \neg P \lor (\neg Q \lor R) \eqv
(\neg P \lor \neg Q) \lor R \eqv \neg (P \land Q) \lor R \eqv (P \land Q) \imp R$$
Laws used:
$$CL \to CL \to ASC \to DML \to CL$$

\subsection*{1.2.8}

\textit{Show that $(P \imp Q) \imp R$ and $P \imp (Q \imp R)$ are not logically equivalent}

We're gonna show that $q \land w \eqv false$
$$((P \imp Q) \imp R) \land (P \imp (Q \imp R)) \eqv (\neg (\neg P \lor Q) \lor R) \land
(\neg P \lor (\neg Q \lor R)) \eqv $$
$$\eqv ((P \land \neg Q) \lor R) \land (\neg P \lor \neg Q \lor R) \eqv
((P \land Q) \land (\neg P \lor \neg Q)) \lor R  \eqv$$
$$ \eqv ((P \land Q) \land \neg ( P \land  Q)) \lor R  \eqv false \lor R \eqv false$$


\section{Predicates and Quantifiers}

\section{A Formal Language for Set Theory}

\subsection{}

\textit{What does the formula $\exists x \forall y (x \notin y)$ say in English? }

There exists $x$ such that for every $y$ we've got that x is not in y. In other ways, there
exists an empty set.

\subsection{}

\textit{What does the formula $\forall y \exists x (y \notin x)$ say in English?}

For every y there exists set x such that y is not in x.

\subsection{}

\textit{What does the formula $\forall y \exists x (x \notin y)$ say in English?}

For every y there exists x such that x is not in y.

\subsection{}

\textit{What does the formula $\forall y \neg \exists x (x \notin y)$ say in English?}

For every y there does not exist an x such that x is not in y.

\subsection{}

\textit{What does the formula $\forall z \exists x \exists y (x \in y \land y \in z)$
  say in English?}

For every $z$ there exists x and y such that x is in y and y is in z

\subsection{}

\textit{Let $\phi(x)$ be a formula. What does $\forall z \forall y((\phi(x) \land \phi(y))
  \to z = y$}

For every z and y, $\phi(x)$ and $\phi(y)$ implies that z = y.

\subsection{}

\textit{Translate each of the following into the language of set theory.}

\textit{(a) x is the union of a and b}

$$\forall (y \in x) (y \in a \land y \in b)$$

\textit{(b) x is not a subset of y}

$$\exists (z \in x) (\neg z \in y)$$

\textit{(c) x is the intersection of a and b}

$$\forall (y \in x) (y \in a \lor y \in b)$$

\textit{(d) a and b have no elements in common}

$$\forall (x \in a) \forall (y \in b) (\neg x = y)$$

\subsection{}

\textit{Let a, b, C and D be sets. Show that the relationship}
$$y =
\begin{cases}
  a \text{ if } x \in C \setminus D \\
  b \text{ if } x \notin C \setminus D \\
\end{cases}
$$

$$((x \in C \land \neg x \in D) \to (y = a)) \land ((\neg x \in C \land \neg x \in D) \to (y = a))$$


\section{The Zermelo-Fraenkel Axioms}

\subsection{}

\textit{Let $u, v, w$ be sets. By pairing axiom, the sets $\{u\}$ and $\{v, w\}$
  exist. Using the pairing and union axioms, show that the set $\{u, v, w\}$
  exists.}

By pairing axiom we've got that
$$PA(u, u) = \{u\}$$
$$PA(v, w) = \{v, w\}$$
thus
$$PA(\{u\}, \{v, w\}) = \{\{u\}, \{v, w\}\}$$
and therefore by union axiom we follow that
$$UA(\{\{u\}, \{v, w\}\}) = \{u, v, w\}$$
as desired.

\subsection{}

\textit{Let $A$ be a set. Show that the pairing axiom implies that the set $\{A\}$ exists}

$$PA(A, A) = \{A, A\}$$
which by extension axiom is equal to $\{A\}$, as desired.

\subsection{}

\textit{Let $A$ be a set. The pairing axiom implies that the set $\{A\}$ exists. Using the
  regularity axiom, show that $A \cap \{A\} = 0$. Conclude that $A \notin A$.}

Since $\{A\} \neq \emptyset$, we follow that there exists $x$ such that $x \in \{A\}$ and
$x \cap \{A\} = \emptyset$. Since $A$ is the only element of $\{A\}$, we follow that
$A \cap \{A\} = \emptyset$, as desired.

\subsection{}

\textit{For sets $A, B$, the set $\{A, B\}$ exists by the pairing axiom. Let $A \in B$.
  Using the regularity axiom, show that $A \cap \{A, B\} = \emptyset$, and thus $B \notin A$.}

$\{A, B\}$ consists of sets $A$ and $B$, thus it is not empty and therefore
there exists $x \in \{A, B\}$ such that $x \in \{A, B\} \land x \cap \{A, B\} = \emptyset$.
For $B$ we've got that $B \in \{A, B\}$. Since $A \in B$ and $A \in \{A, B\}$, we can follow that
$A \in (B \cap \{A, B\})$. By pairing axiom we follow that the element with desired
property must exists, and given that the only other choice is $A$,
we conclude that $A \cap \{A, B\} = \emptyset$. Therefore we can follow that $B \notin A$, as
desired.

\subsection{}

\textit{Let $A, B, C$ be sets. Suppoes that $A \in B$ and $B \in C$. Using the regularity axiom,
  show that $C \notin A$.}

This is an expantion of previous exercise. We can follow that
$$B \in \{A, B, C\} \land B \in C \imp B \in C \cap \{A, B, C\} \imp C \cap \{A, B, C\}
\neq \emptyset$$
$$A \in \{A, B, C\} \land A \in B \imp A \in B \cap \{A, B, C\} \imp B \cap \{A, B, C\}
\neq \emptyset$$
thus the only other choice is $A$, and therefore $A \cap  \{A, B, C\} = \emptyset$. Therefore
$C \notin A$, as desired.


\subsection{}

\textit{Let $A, B$ be sets. Using the subset and power set axioms, show that the set
  $\pow(A) \cap B$ exists.}

Because set $A$ exists we follow that $\pow(A)$ exists. By setting $\phi(x): x \in B$ and
subset axiom we follow that there exists a subset of $\pow(A)$ such that
$x \in S \lra x \in \pow(A) \land x \in B$. Thus we follow by Extensionality axiom
that $S = \pow(A) \cap B$. Thus $\pow(A) \cap B$ exists.

\subsection{}

\textit{Let $A, B$ be sets. Using the subset axiom, show that the set $A \setminus B$ exists.}

$$\phi(x): \neg x \in B$$
thus by subset axiom
$$x \in S \lra x \in A \land \neg x \in B$$
thus $A \setminus B$ exists.

\subsection{}

\textit{Show that no two of the sets $\emptyset, \{\emptyset\}, \{\emptyset, \{\emptyset\}\}$
  are equal to each other.}

I had a little confusion with this one at first because I thought that every set has
empty set in it, which is false. Every set has an empty set as a subset, but it
might be so that empty set is not in the set itself.
$$\emptyset \notin \emptyset \land \emptyset \in \{\emptyset\} \imp \emptyset \neq \{\emptyset\}$$
$$\emptyset \notin \emptyset \land \emptyset \in \{\emptyset, \{\emptyset\}\} \imp
\emptyset \neq \{\emptyset, \{\emptyset\}\}$$
$$\{\emptyset\} \notin \{\emptyset\} \land \{\emptyset\} \in \{\emptyset, \{\emptyset\}\} \imp
\{\emptyset\} \neq \{\emptyset, \{\emptyset\}\}$$
all of the implication follow from extensionality axiom.

\subsection{}

\textit{Let $A$ be a set with no elements. Show that for all $x$, we have that $x \in A$ if
  and only if $x \in \emptyset$. Using the extensionality axiom, conclude that $A = \emptyset$.}

Suppose that $\neg x \in A$. Then we follow that $x$ is an element, therefore $\neg x \in \emptyset$.
Thus
$$\neg x \in A \imp \neg x \in \emptyset \iff x \in \emptyset \imp x \in A$$
Suppose that $\neg x \in \emptyset$. Then we follow that $x$ is an element. Thus $\neg x \in A$.
Thus
$$\neg x \in \emptyset \imp \neg x \in A \iff x \in A \imp x \in  \emptyset$$
thus we follow that
$$x \in \emptyset \lra x \in A$$
thus by extensionality axiom we follow that
$$\emptyset = A$$
which gives us nice follow-up that
$$\emptyset = \{\}$$

\subsection{}

\textit{Let $\phi(x, y)$ be the formula $\forall z(z \in y \lra z = x)$ which asserts that
  $y = \{x\}$. For all x the set $\{x\}$ exists. So $\forall x  \exists! y \phi(x, y)$.
  Let $A$ be a set. Show that the collection $\{\{x\}: x \in A\}$ is a set.}

We know that $A$ is a set and therefore $\pow(A)$ is also a set. Thus by subset axiom
there exists a set 
$$\exists S (x \in S \lra x \in \pow(A) \land \exists(y \in A)(\phi(x, y)))$$
which is precisely our collection.

\chapter{Basic Set-Building Axioms and Operations}

\section{The First Six Axioms}

Prove the following theorems, where $A, B, C, D$ are sets.

\subsection*{2.1.1}

$$A \subseteq B \to (A \subseteq A \cup B \land A \cap B \subseteq A )$$

$$ \forall x (x \in A \to x \in B) \to ((\forall x (x \in A \imp x \in A \lor x \in B)) \land
(\forall (x \in A \land x \in B \imp x \in A))) \lra $$
$$ \lra
\forall x (x \in A \to x \in B) \to ((\forall x (\neg x \in A \lor x \in A \lor x \in B)) \land
(\forall (\neg (x \in A \land x \in B) \lor x \in A))) \lra $$
$$ \lra \forall x (x \in A \to x \in B) \to ((\forall x ( \true  \lor x \in B)) \land
(\forall ( \neg x \in A \lor \neg x \in B \lor x \in A))) \lra $$
$$ \lra \forall x (x \in A \to x \in B) \to (\true \land
(\forall ( true \lor \neg x \in B))) \lra $$
$$ \lra \neg \forall x (x \in A \to x \in B) \lor (\true \land \true) \lra $$
$$ \lra \neg \forall x (x \in A \to x \in B) \lor \true \lra $$
$$\true$$

\subsection*{2.1.2}

$$A \subseteq B \land B \subseteq C \to A \subseteq C$$

$$(\forall x (x \in A \imp x \in B)) \land (\forall x (x \in B \imp x \in C)) \to
\forall x (x \in A \imp x \in C) \lra$$
$$\lra (\forall x (\neg x \in A \lor x \in B)) \land (\forall x (\neg x \in B \lor x \in C)) \to
\forall x (\neg x \in A \lor x \in C) \lra $$
$$\lra (\forall x ((\neg x \in A \lor x \in B) \land  (\neg x \in B \lor x \in C))) \to
\forall x (\neg x \in A \lor x \in C) \lra $$
$$\lra (\forall x ((\neg x \in A \land  (\neg x \in B \lor x \in C))
\lor( x \in B  \land  (\neg x \in B \lor x \in C)))) \to
\forall x (\neg x \in A \lor x \in C) \lra $$
$$\lra (\forall x (\neg x \in A \land  (\neg x \in B \lor x \in C))
\lor( (x \in B  \land  \neg x \in B)  \lor (x \in B  \land x \in C)))) \to
\forall x (\neg x \in A \lor x \in C) \lra $$
$$\lra (\forall x ((\neg x \in A \land  \neg x \in B) \lor (\neg x \in A \land x \in C) 
\lor(  x \in B  \land x \in C)) \to \forall x (\neg x \in A \lor x \in C) \lra  ... $$

So this thing is tedious as hell and should be left to computers.

Suppose that $x \in A$. Then we follow by $A \subseteq B$ that $x \in B$. Thus by $B \subseteq C$
we follow that$x \in C$. Therefore $x \in A \to x \in C$. Therefore $A \subseteq C$, as desired.

\subsection*{2.1.3}

$$B \subseteq C \imp A \setminus C \subseteq A \setminus B$$

Suppose that $x \in A \setminus C$. Then we follow that $x \in A$ and $x \notin C$. Therefore
$x \in A$ and $x \notin B$ since $B \subseteq C$. Thus $x \in A \setminus B$. Therefore
we follow that $B \subseteq C$ implies that  $A \setminus C \subseteq A \setminus B$,
as desired.

\subsection*{2.1.4}

$$C \subseteq A \land C \subseteq B \iff C \subseteq A \cap B$$

Suppose that $x \in C$. Then we follow that $x \in A$ and $x \in B$. Thus $x \in A \cap B$.
Therefore $C \subseteq A \cap B$. Thus we follow that
$C \subseteq A \land C \subseteq B \imp C \subseteq A \cap B$

Suppose that $x \in C$. Then we follow that $x \in A \cap B$. Thus $x \in A$ and $x \in B$.
Therefore $C \subseteq A \land C \subseteq B$. Therefore
$C \subseteq A \cap B \imp C \subseteq A \land C \subseteq B $
thus we follow that
$$C \subseteq A \land C \subseteq B \iff C \subseteq A \cap B$$
as desired.

\subsection*{2.1.5}

\textit{There exists an $x$ such that $x \notin A$}

Suppose that there does not exist $x$ such that $x \notin A$. Then we follow that every set is a
member of $A$, which is impossible.

\subsection*{2.1.6}

$$A \cap B = B \cap A$$

$$x \in A \cap B \iff x \in A \land x \in B \iff x \in B \land x \in A \iff x \in B \cap A$$

\subsection*{2.1.7}

$$A \cup B = B \cup A$$

$$x \in A \cup B \iff x \in A \lor x \in B \iff x \in B \lor x \in A \iff x \in B \cup A$$

\subsection*{2.1.8}

$$A \cap (B \cup C) = (A \cup C) \cap (A \cup B)$$

$$x \in A \cap (B \cup C) \lra  x \in A \land x \in (B \cup C) \lra
x \in A \land (x \in B \lor x \in C) \lra
$$
$$ \lra (x \in A \lor x \in C) \land (x \in A \lor x \in C)
\lra (x \in A \cup B) \lor (x \in A \cup C) \lra x \in ((A \cup B) \cap (A \cup C))$$

\subsection*{2.1.31}

$$A \subseteq \pow(\cup(A))$$

Let $x \in A$. Then we follow that $x \subseteq \cup(A)$. Thus $x \in \pow(A)$. Thus
$A \subseteq \pow(\cup(A))$.

\subsection*{2.1.32}

\textit{Let $C \in F$. Then $\pow(C) \in \pow(\pow(\cup F))$}

Suppose that $C \in F$. Then we follow that $C \subseteq \cup F$. Therefore $C \in \pow (\cup F)$.
Thus $\pow(C) \in \pow(\pow (\cup F))$.


\textit{the rest of the exercises for this section are more of the same.}

\section{Operations on Sets}

Prove the following theorems

\subsection{}

\textit{Let $A$ be a set and $F \neq \emptyset$. Then}
$$A \setminus \cap F = \cup\{A \setminus C: C \in F\}$$

$$x \in A \setminus \cap F \lra
x \in A \land x \notin \cap F \lra
x \in A \land \neg x \in \cap F \lra
x \in A \land \neg (\forall(C \in F)(x \in C)) \lra
$$
$$ \lra
x \in A \land \exists(C \in F)(x \notin C) \lra
\exists(C \in F)(x \notin C \land x \in A) \lra
\exists(C \in F)(x \in A \setminus C) \lra
x \in \cup\{A \setminus C: C \in F\}
$$
which seems to hold.

\subsection{}

\textit{Let $A, F$ be sets. Then $A \cup (\cup F) = \cup\{A \cup C: C \in F\}$}

$$x \in A \cup (\cup F) \lra x \in A \lor x \in \cup F \lra
x \in A \lor  (\exists C \in F)(x \in C) \lra$$
$$
\lra (\exists C \in F)(x \in A) \lor \exists(C \in F)( x \in C) \lra
$$
$$ \lra 
\exists(C \in F)(x \in A \lor x \in C) \lra
\exists(C \in F)(x \in A \cup C) \lra x \in \cup\{A \cup C: C \in F\}
$$

Where we've used the fact that
$$x \in A \lra x \in A \land \true \lra x \in A \land (\exists C \in F)(\true) \lra
(\exists C \in F)(x \in A  \land \true) \lra  (\exists C \in F)(x \in A)$$
don't know if we can use it, but I used it anyways.




\subsection{}

\textit{Let $A, F$ be sets. Then $A \cap (\cup F) = \cup\{A \cap C: C \in F\}$}

$$x \in A \cap (\cup F) \lra x \in A \land x \in \cup F \lra
x \in A \land  (\exists C \in F)(x \in C) \lra$$
$$ \lra 
\exists(C \in F)(x \in A \land x \in C) \lra
\exists(C \in F)(x \in A \cap C) \lra x \in \cup\{A \cap C: C \in F\}$$


\subsection*{2.2.5}

\textit{Let $A$ and $F$ be sets. Then there exists a unique set $\epsilon$ such that for all
  $Y$ we have that $Y \in \epsilon$ if and only if $Y = A \cap C$ for some $C \in F$.}

$\cup F$ exists by union axiom, $A \cap (\cup F)$ exists by subset axiom. Thus $\pow(A \cap (\cup F))$
exists by power axiom. Since $Y = A \cap C \imp Y \subseteq A \cap (\cup F)$, we follow that
$Y$ is a subset of $\pow(A \cap (\cup F))$, which exists by subset axiom. By extensionality axiom we follow that
the set is unique.

\subsection*{2.2.12}

\textit{If $F$ and $G$ are nonempty sets, then }
$$\cap(F \cup G) = \cap(F) \cap  \cap(G)$$

$$x \in \cap(F \cup G) \lra (\forall C \in F \cup G)(x \in C) \lra (\forall C \in F)(x \in C) \land
(\forall C \in G)(x \in C) \lra $$
$$ \lra x \in \cap(F) \land x \in \cap(G) \lra x \in (\cap(F)) \cap (\cap(G))$$


\subsection*{2.2.14}

\textit{Let $F$ be a nonempty set. Then}
$$\pow(\cap (F)) = \cap\{\pow(C): C \in F\}$$

$$x \in \pow(\cap (F)) \lra x \subseteq \cap (F) \lra (\forall y \in x)(y \in \cap (F)) \lra
(\forall y \in x)(\forall (C \in F) (y \in F)) \lra $$
$$
\forall (C \in F) ( (\forall y \in x) y \in F) \lra
\lra \forall(C \in F)(x \subseteq C) \lra \forall(C \in F)(x \in \pow(C)) \lra x \in  \cap\{\pow(C): C \in F\}$$

\chapter{Relations and Functions}

\section{Ordered Pairs in Set Theory}

\subsection{}

\textit{Define $\eangle{a, b, c} = \eangle{\eangle{a, b}, c}$ for any sets $a, b, c$. Prove that this yields an
  ordered tuple; that is, prove tahat if $\eangle{x, y, z} = \eangle{a, b, c}$, then $x = a$, $y = b$, $z = c$.}

Suppose that
$$\eangle{x_1, x_2, x_3} = \eangle{y_1, y_2, y_3}$$
then we follow that
$$\eangle{\eangle{x_1, x_2}, x_3} = \eangle{\eangle{y_1, y_2}, y_3}$$
from which we get that $\eangle{x_1, x_2} = \eangle{y_1, y_2}$ and $x_3 = y_3$. From
$\eangle{x_1, x_2} = \eangle{y_1, y_2}$ we get that $x_1  = y_1$ and $x_2 = y_2$. In
total we get that
$$\eangle{\eangle{x_1, x_2}, x_3} = \eangle{\eangle{y_1, y_2}, y_3}
\imp x_1 = y_1 \land x_2 = y_2 \land x_3 = y_3$$
Thus we follow that given construction defines an ordered tuple, as desired.

\subsection{}

\textit{Prove that $(A \cup B) \times C = (A \times C) \cup (B \times C)$}

$$x \in (A \cup B) \times C \lra x = \eangle{y, z} \land y \in A \cup B \land z \in C
\lra  x = \eangle{y, z} \land (y \in A \lor y \in  B) \land z \in C $$
$$ \lra  (x = \eangle{y, z} \land z \in C ) \land (y \in A \lor y \in  B) \lra $$
$$\lra 
(x = \eangle{y, z} \land z \in C \land y \in A ) \lor
(x = \eangle{y, z} \land z \in C \land y \in B ) \lra$$
$$\lra 
(x \in A \times C ) \lor (x \in B \times C) \lra x \in (A \times C) \cup (B \times C)$$
as desired.

\subsection{}

\textit{Prove that $(A \setminus B) \times C = (A \times C) \setminus (B \times C)$}

$$x \in (A \setminus B) \times C \lra x = \eangle{y, z} \land y \in A \setminus B \land z \in C
\lra  x = \eangle{y, z} \land (y \in A \land y \notin  B) \land z \in C $$
$$ \lra  (x = \eangle{y, z} \land z \in C ) \land (y \in A \land y \notin  B) \lra $$
$$ \lra  x = \eangle{y, z} \land z \in C \land y \in A \land y \notin  B \lra $$
$$ \lra  (x = \eangle{y, z} \land y \in A \land z \in C) \land
 (x \neq \eangle{y, z} \lor y \notin B \lor z \notin C)  \lra $$
$$ \lra  (x = \eangle{y, z} \land y \in A \land z \in C) \land
 (x \neq \eangle{y, z} \lor y \notin B \lor z \notin C)  \lra $$
$$ \lra  (x = \eangle{y, z} \land y \in A \land z \in C) \land
\neg (x = \eangle{y, z} \land y \in B \land z \in C))  \lra $$
$$\lra 
(x \in A \times C) \land \neg (x \in B \times C) \lra x \in (A \times C) \setminus (B \times C)$$

Used a biconditional defined in "useful things"


\subsection{}

\textit{Prove that $$(\cup F) \times C = \cup\{A \times C: A \in F\}$$}

$$x \in (\cup F) \times C \lra x = \eangle{y, z} \land y \in (\cup F) \land z \in C \lra
x = \eangle{y, z} \land (\exists A \in F)(y \in A) \land z \in C \lra
$$
$$ \lra   (\exists A \in F)(y \in A \land x = \eangle{y, z} \land z \in C) \lra
(\exists A \in F)(x \in A \times C) \lra$$
$$\lra x \in  \cup\{A \times C: A \in F\}$$

\section{Relations}

\subsection{}

\textit{Explain why the empty set is a relation}

Relation is defined to be a set of ordered pairs. That is, for every $x \in R$, $x$ is an ordered pair.
Since we haven't got any elements in the emptyset, we follow that the logical statement is true and  therefore
emptyset is a relation.

Other way to see it is to assume that it is not a relation. Then we follow that emptyset has an element that
is not an ordered pair. Since emptyset does not have any elements, we follow that we have
a contradiction.

\subsection{}

\textit{Prove items 1-3 of Theorem 3.2.7}

$$x \in \dom(R \inv) \lra \exists y (\eangle{x, y} \in R \inv)
\lra \exists y (\eangle{y, x} \in R) \lra x \in \ran(R)$$

$$x \in \ran(R \inv) \lra \exists y (\eangle{y, x} \in R \inv)
\lra \exists y (\eangle{x, y} \in R) \lra x \in \dom(R)$$

$$x \in (R \inv) \inv \lra \exists y \exists z (\eangle{y, z} \in (R \inv) \inv ) \land x = \eangle{y, z}
\lra \exists y \exists z (\eangle{z, y} \in (R \inv) ) \land x = \eangle{y, z} \lra $$
$$ \lra  \exists y \exists z (\eangle{y, z} \in R ) \land x = \eangle{y, z} \lra x \in R$$


\subsection*{3.2.4}

$$\dom(R) = \{0, 1, 2, 3, 4\}$$
$$\ran(R) = \{0, 1, 2, 3, 4\}$$
$$R \circ R = \{\eangle{0, 2}, \eangle{0, 3}, \eangle{0, 0}, \eangle{0, 3}, \eangle{0, 4},
\eangle{1, 0}, \eangle{1, 3}, \eangle{1, 4}, \eangle{1, 3}, \eangle{1, 2}, \eangle{2, 1},$$
$$ 
\eangle{2, 2}, \eangle{2, 3}, \eangle{2, 2}, \eangle{2, 4}, \eangle{3, 3}, \eangle{3, 2},
\eangle{4, 4}\}$$
$$R|\{1\} = \{\eangle{1, 2}, \eangle{1, 3}\}$$
$$R\inv|\{1\} = \{\eangle{1, 0}\}$$
$$R[\{1\}] = \{2, 3\}$$
$$R\inv[\{1\}] = \{0\}$$

\subsection*{3.2.5}

\textit{Suppose that $R$ is a relation. Prove that $R|(A \cup B) = (R | A) \cup (R | B)$
  for any sets $A, B$}

$$x \in R|(A \cup B) \lra (\exists y \in A \cup B) (\exists z \in  \ran(R)) (\eangle{y, z}
\in R \land x = \eangle{y, z}) \lra $$
$$ 
\lra (\exists y \in A) (\exists z \in  \ran(R)) (\eangle{y, z}
\in R \land x = \eangle{y, z}) \lor
 (\exists y \in B) (\exists z \in  \ran(R)) (\eangle{y, z}
\in R \land x = \eangle{y, z}) \lra $$
$$ \lra x \in R|A \lor x \in R|B \lra x \in (R|A \cup R|B)$$
thus
$$R|(A \cup B) = (R | A) \cup (R | B)$$
as desired.

\subsection*{3.2.7}

\textit{Let $R$ and $S$ be two relations and let $A, B, C$ be sets. Prove that $R|A$,
  $R\inv [B]$, $R[C]$ and $R \circ S$ are sets.}

Given that $R$ and $S$ are relation, we follow that both of them are sets,
$\bigcup \bigcup R$ and  $\bigcup \bigcup S$ are sets and $\dom (R), \ran(R), \dom(S), \ran(S)$
are sets. Thus we follow that $R|A$ is a subset of
$R$, which is a set; $R\inv [B]$  and $R[C]$ are subsets of $\bigcup \bigcup R$,
and $R \circ S$ are subsets of a set $\dom (R) \times \ran(S)$, which is a set.


\subsection*{3.2.8}

\textit{Let $R$ be a relation and $G$ be a set. Prove that $\{R[C]: C \in G\}$ is a set. Prove
  that if $G$ is nonempty, then $\{R[C]: C \in G\}$ is also nonempty}

If $R$ is a relation, then $\ran(R)$ is a set. Therefore $\pow(\ran(R))$ is a set. Thus
for any set $C$, $R[C] \subseteq \ran(R)$, therefore $R[C] \in \pow(\ran(R))$. Thus
$\{R[C]: C \in G\}$ is a subset of $\pow(\pow(\ran(R)))$, which is a set.

Suppose that $G$ is nonempty. Then we follow that there exists $C \in G$. Thus
$R[C]$ is a set. Thus $R[C] \in \{R[C]: C \in G\}$. Therefore $\{R[C]: C \in G\}$ is
nonempty.

\subsection*{3.2.19}

\textit{Prove item (2) of Theorem 3.2.8}

$$R[\bigcup G] = \bigcup{R[C]: C \in G}$$

$$x \in R[\bigcup G] \lra (\exists y \in \bigcup G)(\eangle{y, x} \in R) \lra
(\exists C \in G)(y \in C \land \eangle{y, x} \in R) \lra$$
$$\lra (\exists C \in G)(x \in R[C]) \lra x \in \bigcup{R[C]: C \in G}$$

\subsection*{3.2.20}

\textit{Prove item (4) fo Theorem 3.2.8}

$$x \in R[\bigcap G] \lra (\exists y \in \bigcap G)(\eangle{y, x} \in R) \lra
\exists y (\forall C \in  G)( y \in C \land \eangle{y, x} \in R) \ra$$
$$ \ra
(\forall C \in G) (\exists y \in C) ( \eangle{y, x} \in R) \lra
(\forall C \in G) (x \in R[C]) \lra x \in \bigcap{\{R[C]: C \in G\}}$$

\section{Functions}

\subsection*{3.3.1}

\textit{Prove Lemma 3.3.5 and Lemma 3.3.13}

Suppose that $F$ and $G$ are functions such that $\dom(F) = \dom(G)$. 
Lemma 3.3.5 states that $F = G$ iff $F(x) = G(x)$ for every $x \in \dom(F)$
If $F = G$, then
$$F(x) = y \lra \eangle{x, y} \in F \lra \eangle{x, y} \in G \lra G(x) = y$$
thus $F(x) = G(x)$ for every $x \in \dom(F)$.

Now suppose that $F(x) = G(x)$ for every $x \in \dom(F)$. Then we follow that
$$z \in F \lra z = \eangle{x, y} \land F(x) = y \lra
z = \eangle{x, y} \land G(x) = y \lra z \in G$$
as desired.

Lemma 3.3.13 states that a function $F$ is one-to-one if and only if $F$ is single-rooted.

Suppose that $F$ is one-to-one and $F$ is not single rooted. Then we follow that
there exists $x, y \in F$ such that $x = \eangle{u, w} \in F, y = \eangle{j, w} \in F$.
Then we follow that $F(u) = w = F(j)$, which is a contradiction.

Proof of converse is extremely simular.

\subsection*{3.3.2}

\textit{Let $F$ be a function and let $A \subseteq B \subseteq \dom(F)$. Prove that
  $F[A] \subseteq F[B]$.}

$$x \in F[A] \lra x = \eangle{u, v} \land u \in A \land \eangle{u, v} \in F \ra
x = \eangle{u, v} \land u \in B \land \eangle{u, v} \in F \lra x \in F[B]$$

\subsection*{3.3.5}

\textit{Let $g: C \to D$ be a one-to-one function, $A \subseteq C$ and $B \subseteq C$. Prove
  that if $A \cup B = \emptyset$, then $g[A] \cap g[B] = \emptyset$.}

Suppose that $A \cap B = \emptyset$ and $g[A] \cap g[B] \neq \emptyset$. Then we follow that
there exists $x \in g[A] \cap g[B]$. Thus
$$x \in g[A] \land x \in g[B] \lra (\exists y \in A)(\eangle{y, x} \in g) \land
(\exists z \in B)(\eangle{z, x} \in g)$$
since $g$ is one-to-one, we follow that $z = y$. Thus there exists $z \in A \cap B$, therefore
$A \cap B \neq \emptyset$, which is a contradiction.

\subsection*{3.3.9}

\textit{Suppose that $F: X \to Y$ is a function. Prove that if $C \subseteq Y$ and
  $D \subseteq Y$, then $F\inv[C \cap D] = F\inv[C] \cap F\inv[D]$.}

Since $F$ is a function, we follow that $F\inv$ is a single-rooted relation. Thus we follow that
$$F\inv[C \cap D] = F\inv[C] \cap F\inv[D]$$
as desired.

\subsection*{3.3.10}

\textit{Let $F, G$ be functions from $A$ to $B$. Suppose $F \subseteq G$. Prove that $F = G$.}

Suppose that $x \in A$. Then we follow that
$$(\exists y \in B)(\eangle{x, y} \in F) \ra (\exists y \in B)(\eangle{x, y} \in G)$$
Thus we follow that for every $x \in A$ (where $\dom (F) = A = \dom(G)$)
$$F(x) = G(x)$$
thus by the lemma 3.3.5 we follow that
$$F = G$$
as desired.


\subsection*{3.3.11}

\textit{Let $C$ be a set of functions. Suppose that for all $f$ and $g$ in $C$, we have either
  $f \subseteq g$ or $g \subseteq f$. }

\textit{(a) Prove that $\cup C$ is a function}

Firstly, since $C$ is a set of sets of ordered pairs, we follow that $\cup C$ is a set of
ordered pairs, and therefore it is a relation. Suppose that $x \in \cup C$. Then we follow that
there exist  $f \in C$ such that $x \in f$ and 
$x = \eangle{u, v}$. Suppose that there exists $y \in \cup C$, such that $y = \eangle{u, v'}$,
where $u' \neq u$. Since $y \in \cup C$, we follow that there exists $g \in C$ such that
$y \in C$. Because $u' \neq u$, we follow that $g \neq f$. Therefore either $g \subset f$,
or $f \subset g$. In both cases we follow that we can't have the case that $u' \neq u$. Thus
we follow that for $x, y \in \cup C$, whenever the first part of the $x$ is equal to the first
part of $y$, we follow that the last parts are also equal. Thus we follow that $\cup C$ is
a single-valued relation, and therefore it is a function.

\subsection*{3.3.13}

\textit{Assume $f: A \to B$ is onto $B$. Let $C \subseteq B$. Prove that $f[f\inv[C]] = C$}

$$x \in f[f\inv[C]] \lra (\exists y \in f\inv[C])(f(y) = x) \lra
(\exists z \in C)(\eangle{y, z} \in f \land f(y) = x) \lra$$
$$ \lra (\exists z \in C)(f(y) = z \land f(y) = x) \lra (\exists z \in C)(x = z) \lra x \in C$$
this notation may be a bit sloppy, but the result is derived faithfully.

\subsection*{3.3.15}

\textit{Let $f: A \to B$ be a one-to-one function. Define $G: \pow(A) \to \pow(B)$ by
  $G(X) = f[X]$, for each $X \in \pow(A)$. Prove that $G$ is one-to-one.}

Let $X_1, X_2 \in \pow(A)$ be such that $G(X_1) = G(X_2)$. Then we follow that
$$f[X_1] = f[X_2]$$
thus
$$x \in X_1 \lra (\exists y \in f[X_1])(\eangle{x, y} \in f) \lra
(\exists y \in f[X_2])(\eangle{x, y} \in f) \lra x \in X_2$$
thus we follow that $X_1 = X_2$. Therefore $G(X_1) = G(X_2) \to X_1 = X_2$, thus $G$ is
one-to-one, as desired.

\subsection*{3.3.21}

\textit{Let $\eangle{A_i: i \in I}$ be an indexed function with nonempty terms. Prove that there
  is an indexed function ${x_i: i \in I}$ si that $x_i \in A_i$ for all $i \in I$, using
  theorem 3.3.24}

TODO



\end{document}
%%% Local Variables:
%%% mode: latex
%%% TeX-master: t
%%% End:
