\documentclass[11pt,oneside,titlepage]{report}
\title{My linear algebra exercises}
% \usepackage{amsmath,amssymb}
% \usepackage{geometry}
\author{Evgeny Markin}
\date{2022}

\begin{document}
\maketitle
\tableofcontents

\chapter*{Preface}

Exercises are from "Linear algebra done right" by Sheldon Axler, 3rd ed.
I've already read this book before and completed some exercises from it.
Right now I want to brush up the material once again, put all the
proofs on a more durable material than paper and to prepare myself to
what's gonna happen afterwards.

\chapter{1.A $R^n$ and $C^n$}

\section*{1}
\textit{Suppose $a$ and $b$ are real numbers, not both $0$. Find real nuber
  $c$ and $d$ such that }
$$1/(a + bi) = c + di$$

$$\frac{1}{a + bi} = c + di$$
$$\frac{1}{a + bi} - c - di = 0$$
$$\frac{a - bi}{(a + bi)(a - bi)} = c + di$$
$$\frac{a - bi}{(a^2 + b^2)} = c + di$$
$$\frac{a}{a^2 + b^2} - \frac{b}{a^2 + b^2}i = c + di$$
Thus $c = \frac{a}{a^2 + b^2}$ and $d = -\frac{b}{a^2 + b^2}$

\section*{2}
\textit{Show that }
$$\frac{-1  + \sqrt{3}i}{2}$$
\textit{is a cube root of $1$ (meaning that its cube equals 1)}
$$(\frac{-1  + \sqrt{3}i}{2})^3 =
\frac{(-1  + \sqrt{3}i)^3}{8} =
\frac{(-1  + \sqrt{3}i)(-1  + \sqrt{3}i)^2}{8} =
\frac{(-1  + \sqrt{3}i)(1  - 2\sqrt{3}i - 3)}{8} =
$$
$$
=\frac{(-1  + \sqrt{3}i)(-2  - 2\sqrt{3}i)}{8} =
\frac{2 + 2\sqrt{3}i - 2\sqrt{3}i + 6}{8} =
\frac{8}{8} = 1
$$
as desired.

\section*{3}
\textit{Find two distinct square roots of $i$}

Square root of $i$, I assume, is a number, whose square is equal to $i$.
Suppose that $(a + bi)^2 = i$. It follows that
$$(a + bi)^2 = a^2 + 2abi - b^2$$
So if we set $$a = b = 1/\sqrt{2}$$ this equation holds. Also it holds for
$$a = b = -1/\sqrt{2}$$
maxima seems to agree with me on this one

\section*{4}
\textit{Show that $\alpha + \beta = \beta + \alpha$ for all
  $\alpha, \beta \in \textbf{C}$}

Let $\alpha = a_1 + b_1 i$ and $\beta = a_2 + b_2 i$. It follows
$$\alpha + \beta = a_1 + b_1 i + a_2 + b_2 i = a_2 + b_2 i + a_1 + b_1 i =
\beta  + \alpha$$
as desired.

\section*{5}
\textit{Show that $(\alpha + \beta) + \lambda = \alpha + (\beta + \lambda)$
  for all  $\alpha, \beta, \lambda \in \textbf{C}$}

Let $\alpha = a_1 + b_1 i$ , $\beta = a_2 + b_2 i$, $\lambda = a_3 + b_3 i$.
It follows that 
$$\alpha + (\beta + \lambda)  = a_1 + b_1 i + (a_2 + b_2 i + a_3 + b_3 i) =
(a_1 + b_1 i + a_2 + b_2 i) + a_3 + b_3 i = 
(\alpha + \beta) + \lambda$$

\section*{6}
\textit{Show that $(\alpha \beta) \lambda = \alpha( \beta \lambda)$}

$$\alpha + (\beta + \lambda)  = (a_1 + b_1 i) ((a_2 + b_2 i) + (a_3 + b_3 i)) =
((a_1 + b_1 i)(a_2 + b_2 i)) + (a_3 + b_3 i) = 
(\alpha \beta) \lambda$$

\section*{7}
\textit{Show that for every $\alpha \in \textbf{C}$ there exists a unique
  $\beta \in \textbf{C}$ such that $\alpha + \beta = 0$}

Suppose that there exist two different $\beta_1 \neq \beta_2$ such that
$\alpha + \beta_1 = 0$ and $\alpha + \beta_2 = 0$. It follows that
$$ \beta_1 = \beta_1 + 0 =  \beta_1 + \alpha + \beta_2 = \alpha + \beta_1  + \beta_2 = 0  + \beta_2 = \beta_2$$
which is a contradiction. Therefore there exists only one unique $\beta$.

\section*{8}
\textit{Show that for every $\alpha \in \textbf{C}$ with $\alpha \neq 0$
  there exists a unique $\beta \in \textbf{C}$ such that $\alpha \beta = 1$}

Suppose that it is not true and there exist two different
$\beta_1 \neq \beta_2$ such that
$$\alpha \beta_1 = 1 \textit{ and } \alpha \beta_2 = 1$$
it follows then that 
$$\beta_1 = 1 *  \beta_1 = \alpha \beta_2 \beta_1  =
\alpha \beta_1 \beta_2 = 1 * \beta_2 = \beta_2$$
which is a contradiction. Therefore there exists only one unique $\beta$.

\section*{etc}
The rest of the section is the repetition of this kind of stuff.
That is a lot of writing, and not a lot of thinking, so I'll skip it.
I don't ususally like to skip sections, but I have  aa feeling, that I've
completed this thing on paper somewhere, and there is not much reason to
rewrite it here.

\chapter{1B Definition of Vector Space}





\end{document}