\documentclass[11pt,oneside,titlepage]{book}
\title{My real analysis exercises}
\usepackage{amsmath, amssymb}
\usepackage{geometry}
\usepackage{hyperref}
\author{Evgeny Markin}
\date{2022}

\DeclareMathOperator\erf{erf}

\begin{document}
\maketitle
\tableofcontents

\chapter{Differentiation}

\section{Standard differentiation}

\subsection{}

$$g(x) = 4x + 7$$
$$g'(x) = 4$$

\subsection{}

$$g(x) = 5x + 4x^2$$
$$g'(x) = 5 + 8x$$

\subsection{}

$$f(x) = x^{75} - x + 3$$
$$f'(x) = 75 x^{74} - 1$$

\subsection{}

$$g(x) = 7/4 x^2 - 3x + 12$$
$$g'(x) = 7/2 x - 3$$

\subsection{}

$$f(t) = -2e^t$$
$$f'(t) = -2te^t$$

\subsection{}

$$F(t) = t^2 + e^3$$
$$F(t) = 2t + 3e^3$$

\subsection{}

$$ y = (4x^2 + 3)(2x + 5) $$
$$ y' = 8x(2x + 5) + 2(4x^2 + 3) $$

\subsection{}

$$y = x^3 e^x $$
$$y = 3x^2 e^x + x^3 e^x$$

\subsection{}

$$f(x) = (3x^2 - 5x) e^x$$
$$f'(x) = (6x - 5) e^x + (3x^2 - 5x) e^x$$

\subsection{}

$$f(x) = x \cos x \sin x$$
$$f'(x) =  \cos x \sin x - x \sin^2 x + x \cos^2 x$$

\section{Inverse trigonometric and logarythmic integration}

\subsection{}

$$f(x) = \ln(3 + x^2)$$
$$f'(x) = \frac{2x}{3 + x^2}$$

\subsection{}

$$f(x) = \ln (x^2 + 3x + 5)$$
$$f'(x) = \frac{2x + 3}{x^2 + 3x + 5}$$

\subsection{}

$$f(x) = x \ln x - x$$
$$f'(x) = \ln x + 1 - 1 = \ln x$$

\subsection{}

$$f(x) = \sin  (\ln x)$$
$$f'(x) = \cos (\ln x) \frac 1 x$$

\subsection{}

$$f(x) = \ln (\sin^2 x)$$
$$f'(x) = \frac{2 \sin x \cos x}{ \sin^2 x } = \frac{2 \cos x}{ \sin x }$$

\subsection{}

$$f(x) = \ln \frac 1 x$$
$$f'(x) = x (- x^{-2}) = - \frac{1}{x}$$

\subsection{}

$$f(x) = \frac{1}{\ln x}$$
$$f'(x) = - \frac{1}{(\ln x)^2 x} $$

\subsection{}

$$g(x) = \ln (x e^{-2x})$$
$$g'(x) = \frac{e^{-2x} -2xe^{-2x}}{x e^{-2x}}$$

\subsection{}

$$g(t) = \sqrt{1 + \ln t}$$
$$g'(t) = \frac{1}{2t \sqrt{1 + \ln t} }$$

\subsection{}

$$f(t) = (\ln t)^2 \sin t$$
$$f'(t) = 2 \ln t \frac 1 t \sin t + \cos t (\ln t)^2$$

\subsection{}

$$f(t) = \ln (\sqrt{t^2 + 1})$$
$$f'(t) = \frac{2t}{2( t^2 + 1)} = \frac{t}{t^2 + 1}$$

\subsection{}

$$f(x) = \log_8{(x^2 + 3x)}$$
$$f'(x) = \frac{2x + 3}{\ln (8) (x^2 + 3x)}$$

\subsection{}

$$f(x) = \sin^{-1}(5x)$$
$$f'(x) = \frac{5}{\sqrt{1 - (5x)^2}}$$

\subsection{}

$$f(x) = \sec^{-1}(e^x)$$
$$f'(x) = \frac{2 e^{2x}}{e^x \sqrt{e^{2x} - 1}}$$

\subsection{}

$$ f(x) = \tan^{-1}(\sqrt{x - 1})$$
$$ f'(x) = \frac{1}{2 \sqrt{x - 1}(1 + |x - 1|)}$$

\subsection{}

$$f(x) = \tan^{-1}(x^2) $$
$$f'(x) = \frac{2x}{1 + x^4}$$

\subsection{}

$$f(x) = (\tan^{-1}x)^2$$
$$f'(x) = \frac{2(\tan^{-1}x)}{1 + x^2}$$

\subsection{}

$$f(x) = \arccos\sqrt{x}$$
$$f'(x) = \frac{1}{2 \sqrt{x} \sqrt{1 - |x|}}$$

\subsection{}

$$f(x) = (\arcsin x) \ln x$$
$$f'(x) = \frac{\ln x}{\sqrt{1 - x^2}} + \frac{\arcsin x}{x}$$


\subsection{}

$$ f(x) = \ln(\arctan(x^4))$$
$$ f'(x) = \frac{4 x^3}{(1 + x^8)\arctan x^4}$$

\subsection{}

$$f(x) = e^{\arcsin(x^2)}$$
$$f'(x) = e^{\arcsin(x^2)}\frac{2x}{\sqrt{1 - x^4}}$$


\chapter{Basic integration}

\section{Basic integrals}

\subsection{}
$$\int_1^3{(x^2 + 2x - 4)dx} =
[\frac{x^3}{3} + x^2 - 4x]_1^3 = (9 + 9 - 12) - (1/3 + 1 - 4) = 6 + \frac{8}{3} = \frac{26}{3}$$

\subsection{}
\textit{The error function}
$$\erf(x) = \frac{2}{\sqrt{\pi}}\int_0^x{e^{-t^2}dt}$$

\textit{(a) Show that }
$$\int_a^b{e^{-t^2}dt} = \frac{1}{2} \sqrt{\pi} [\erf(b) - \erf(a)]$$

$$\erf(x) = \frac{2}{\sqrt{\pi}}\int_0^x{e^{-t^2}dt}$$
$$\frac{\sqrt{\pi} }{2} \erf(x) = \int_0^x{e^{-t^2}dt}$$
$$\frac{\sqrt{\pi} }{2} \erf(a) = \int_0^a{e^{-t^2}dt}$$
$$\frac{\sqrt{\pi} }{2} \erf(b) - \frac{\sqrt{\pi} }{2} \erf(a) =
\int_0^b{e^{-t^2}dt} - \int_0^a{e^{-t^2}dt}$$
$$\frac{\sqrt{\pi} }{2} \erf(b) - \frac{\sqrt{\pi} }{2} \erf(a) =
\int_0^b{e^{-t^2}dt} + \int_a^0{e^{-t^2}dt}$$
$$\frac{\sqrt{\pi} }{2} \erf(b) - \frac{\sqrt{\pi} }{2} \erf(a) =
\int_a^b{e^{-t^2}dt}$$
$$\frac{1}{2} \sqrt{\pi}  [\erf(b) - \erf(a)] = \int_a^b{e^{-t^2}dt}$$

\textit{(b) Show that the function $y = e^{x^2}\erf(x)$ satisfies the differential equation
  $$y' = 2xy + 2 / \sqrt{\pi}$$}

$$y' = 2x e^{x^2} \erf(x) + e^{x^2} \frac{2}{\pi} e^{-x^2} =
2x e^{x^2} \erf(x) +  \frac{2}{\pi}
$$

$$2xy + 2/\sqrt \pi = 2x e^{x^2}\erf(x) + 2/\sqrt \pi$$
as desired.

\section{Substitution}

\subsection{}
$$\int{\cos 2x dx}$$
$$u = 2x$$
$$\int{\cos 2x dx} = \int{\frac 1 2 2 \cos 2x dx} = \int{\frac 1 2 \cos u du} =
\frac 1 2  \int{\cos u du} = 
\frac 1 2 \sin u = \frac 1 2 \sin 2x$$

\subsection{}

$$\int{x e^{-x^2}dx} =
\int{(- \frac 1 2) -2 x e^{-x^2}dx} =
- \frac 1 2 \int{  e^{u}dx} = - \frac 1 2 e^u = - \frac 1 2 e^{-x^2}
$$

\subsection{}

$$\int{x^2 \sqrt{x^3 + 1}dx} =
\int{\frac{1}{3} 3 x^2 \sqrt{x^3 + 1}dx} =
\frac{1}{3} \int{ \sqrt{u}dx} = \frac{1}{3} u^{3/2} \frac 2 3 = \frac 2 9 (x^3 + 1)^{3/2}
$$

\subsection{}

$$\int{\sin^2 x \cos x} =
\int {u^2} = \frac {u^3} 3= \frac {\sin x} 3
$$

\section{Integration by parts}

\subsection{}

$$ \int {x e^{2x}} =
 x \frac 1 2 e^{2x} - \int {\frac 1 2 e^{2x}} =  \frac 1 2  x e^{2x} - \frac 1 2 e^{2x} 
$$


\end{document}

