\documentclass[11pt,oneside,titlepage]{book}
\title{My algorithms exercises}
\usepackage{amsmath,amssymb}
\usepackage{geometry}
\usepackage{hyperref}
\author{Evgeny Markin}
\date{2022}

\begin{document}
\maketitle
\tableofcontents

\chapter*{Preface}
Exercises for Introduction to Algorithms by Cormen et al., 4th ed. It has some
exercises, that should be written down, moslty in math and whatnot.

\part{Appendix: Mathematical Background}
\chapter{Summations}

\section*{1-1}
\textit{Prove that $\sum_{k  = 1}^n{O(f_k(i))} = O(\sum_{k  = 1}^n{f_k(i)})$}

Short answer:
$$\sum cg(x) = c\sum{g(x)}$$

Long answer:

Suppose that $g \in O(f_k(i))$. It follows that there exists $n_i$ and $c_i$
such that $0 \leq g(n) \leq cf_i(n)$. Thus we can pick
$n = \max\{n_0, n_1, ...\}$ and $c = \max\{c_0, c_1, ... \}$. We know that
both $n$ and $c$ will work all of functions $f_k$. Therefore by
linearity of summations
$$\sum_{k  = 1}^n{O(f_k(i))}
= \sum_{k  = 1}^n{cf_k(i)} =
= c\sum_{k  = 1}^n{f_k(i)} = 
= O(\sum_{k  = 1}^n{f_k(i)})$$
(notation is a little abused and there is nothing is rigorously
proven, but it'll do).

\section*{1-2}
\textit{Find a simple formula for $\sum_{k = 1}^n{(2k - 1)}$.}

$$\sum_{k = 1}^n{(2k - 1)} =
\sum_{k = 1}^n{(2k)} - \sum_{k = 1}^n{(1)} =
2\sum_{k = 1}^n{(k)} - n =
2\frac{n(n + 1)}{2} - n =
n(n + 1) - n =
n^2
$$


\section*{1-3}
\textit{Interpret the decimal number $111,111,111$ in light of equation A.6}

$$111,111,111 = \sum_{k = 0}^{9}{10^k} = \frac{10^{10} - 1}{10 - 1}$$

\section*{1-4}
\textit{Evaluate the infinite series $1 - \frac 1 2 + \frac 1 4 - \frac 1 8
  + \frac{1}{16} - ...$}

The series converges absolutely to 2, so we are free to do anything with it.

$$1 - \frac 1 2 + \frac 1 4 - \frac 1 8
+ \frac{1}{16} - ... = 
\sum_{k = 0}^{\infty}{\frac{1}{2}^{2k}}
- \sum_{k = 0}^{\infty}{\frac{1}{2}^{1 + 2k}} =
\sum_{k = 0}^{\infty}{\frac{1}{2}^{2k}}
- \frac{1}{2}\sum_{k = 0}^{\infty}{\frac{1}{2}^{2k}} =
\left(1 - \frac{1}{2}\right)\sum_{k = 0}^{\infty}{\frac{1}{2}^{2k}} = 
$$
$$
= \left(1 - \frac{1}{2}\right)\sum_{k = 0}^{\infty}{\frac{1}{4}^{k}}
= \left(1 - \frac{1}{2}\right)\frac{1}{1 - \frac{1}{4}}
= \frac 1 2 *  \frac 4 3 = \frac 2 3
$$

\section*{1.5}
\textit{Let $c \geq 0$ be a constant. Show that
  $\sum_{k = 1}^{n}{k^c} = \Theta(n^{c + 1})$}

$$\Theta(\sum_{k = 1}^{n}{k^c}) =
\sum_{k = 1}^{n}{\Theta(k^c)} = 
$$

\section*{1-9}
\textit{Show that $\sum_{k = 0}^{\infty}{(k - 1)/2^k} = 0$}

$$\sum_{k = 0}^{\infty}{(k - 1)/2^k} =
\sum_{k = 0}^{\infty}{(k - 1)/2^k} =
\sum_{k = 1}^{\infty}{(k - 1)/2^k} - \frac{1}{2^0}=
\sum_{k = 1}^{\infty}{(k - 1)/2^k} - 1= 
$$

\end{document}